added a bunch of useful declarations and thms. many to be proven still

CContext.v
@@ -2,18 +2,21 @@ Require Import List.
 Import ListNotations.
 Require Import String.
 Require Import Maps.
+Require Import Omega.
 
 Definition stack (A: Type) := list A.
+Definition frame := stack nat.
+Definition cstack := stack (frame).
 
 (* underlying C specification does not insist on an actual heap *)
-Definition heap := list nat.
+Definition cheap := list nat.
 
 (* We want a way to look up values in the stack and heap.
    We'll have two symbol tables.  One to index into stack values,
 and one to index into heap values
  **)
 
-Definition sym_tbl := total_map nat.  (* make sure to initialize with error default value *) 
+Definition sym_tbl := partial_map nat.  (* make sure to initialize with error default value *) 
 
 (* C programs will be manipulating stack, heap, and symbol table 
  
@@ -22,29 +25,234 @@ Definition sym_tbl := total_map nat.  (* make sure to initialize with error defa
 
 (* TODO - must fix **)
 Inductive context :=
-| space (s: stack nat) (st: sym_tbl) (h: heap) (ht: sym_tbl).
+| space (s: cstack) (st: stack sym_tbl) (h: cheap) (ht: sym_tbl).
 
 (* Some useful properties of our stack, heap, symbol table, and context **)
 
-Definition push {A: Type} (x: A) (xl: stack A): stack A :=
+(* Helpful to do global lookups across stacks **)
+Definition flatten {A: Type} (l: list (list A)): list A :=
+  fold_left (fun la la' => la ++ la') l [].
+
+
+Definition push {A: Type} (xl: stack A) (x: A): stack A :=
   x::xl.
 
-Definition pop {A: Type} (xl: stack A): option (A*stack A) :=
+Definition pop {A: Type} (xl: stack A) (d: A):=
   match xl with
-  | [] => None
-  | h::t => Some (h,t)
+  | [] => (d, [])
+  | h::t => (h,t)
   end.
 
-Definition lookup_s (ctx: context) (var: string) :=
-  let '(space s st _ _) := ctx in
-  let result := st var in
-  nth result s 0.
+Fixpoint get_pred (s: cstack) :=
+  match s with
+  | [] => 100 (* num allowed variables **)
+  | h::t => (get_pred t) - (List.length h)
+  end.
 
-Definition lookup_h (ctx: context) (var: string) :=
-  let '(space _ _ h ht) := ctx in
-  let result := ht var in
-  nth result h 0.
+(*Use this to enter a new scope.  Don't forget that main has a scope **)
+Definition push_new_frame (s: cstack) (st: stack sym_tbl) :=
+  let s' := push s [] in
+  let st' := push st (empty) in
+  (s', st').
 
-Definition lookup (ctx: context) (var: string) :=
-  lookup_s ctx var \/ lookup_h ctx var.
+(*Use this to create new variables on the stack *)
+Definition push_var (s: cstack) (st: stack sym_tbl) (var: string) (v: nat) :=
+  match s, st with
+  | shead::stail, sthead::sttail =>
+    let next_val := get_pred s in
+    let s' := (push shead v)::stail in
+    let st' := (var !-> Some next_val; sthead)::sttail in
+    (s', st')
+  | _, _ => ([], []) (* error case -> always have stack frames **)
+  end.          
+
+(*Use this to return from a scope **)
+Definition pop_frame (s: cstack) (st: stack sym_tbl) :=
+  let '(f, s') := pop s [] in
+  let '(ft, st') := pop st (empty) in
+  (f, s', ft, st').
+
+Fixpoint search_sm (st: stack sym_tbl) (var: string) :=
+  match st with
+  | [] => 0 (* guaranteed lookup success **)
+  | h::t => match h var with
+            | None => search_sm t var
+            | Some n => n
+            end
+  end.
+
+Fixpoint frame_nth (s: cstack) (offset: nat) :=
+  match s with
+  | [] => 0 (* Not going to happen **)
+  | h::t => (fix frame_aux l n :=
+               match l, n with
+               | h'::t', S n => frame_aux t' n
+               | [], _ => frame_nth t n
+               | h'::t', 0 => h'
+               end
+            ) h offset
+  end.
+
+(*Use this to lookup a variable (scope shadowing applies **)
+(*Not efficient.  but it does the job **)
+Definition lookup_s (s: cstack) (st: stack sym_tbl) (var: string) :=
+  let index := search_sm st var in
+  let offset := index - S (get_pred s) in
+  frame_nth s offset. (* guaranteed lookup success here too **)
+
+Definition lookup_h (h: cheap) (ht: sym_tbl) (var: string) :=
+  match ht var with
+  | Some index => nth index h 0
+  | None => 0 (* guaranteed lookup success **)
+  end.
+
+(* Now some useful lemmas **)
+                                                            
+(* Lemma saying that we add to stack properly -decrement by 1 eac time**)
+Lemma add_stack_properly: forall (s s': cstack) (st st': stack sym_tbl) (var: string) (val: nat),
+    s <> [] /\ st <> [] ->
+    get_pred s <> 0 ->
+    push_var s st var val = (s', st') ->
+    get_pred s' = pred (get_pred s).
+Proof.
+  destruct s; intros.
+  inversion H1; subst.
+  destruct H. contradiction.
+
+  inversion H1; subst.
+  destruct st. destruct H; contradiction.
+
+  inversion H3; subst. clear H3.
+  unfold push.
+
+  unfold get_pred.
+
+  simpl.  omega.
+Qed.
+
+Fixpoint stack_size (s: cstack) :=
+  match s with
+  | [] => 0
+  | h::t => (List.length h) + (stack_size t)
+  end.
+
+Lemma add_stack_invariant: forall (s: cstack),
+    s <> [] ->
+    List.length s <= 100 ->
+    get_pred s = 100 - stack_size s.
+Proof.
+  induction s; intros.
+  contradiction.
+
+  destruct s.
+  unfold get_pred.
+  unfold stack_size.
+  omega.
+
+  unfold get_pred, stack_size.
+  assert (get_pred (f :: s) = 100 - stack_size (f :: s)).
+  apply IHs. intros contra. inversion contra.
+  simpl. simpl in H0. omega.
+
+  unfold get_pred, stack_size in H1. omega.
+Qed.
+  
+
+(* Second, when you add a variable, you can get the variable **)
+Lemma add_stack_vars: forall (s s': cstack) (st st': stack sym_tbl)
+                                 (var: string) (val: nat),
+    s <> [] /\ st <> [] ->
+    get_pred s <> 0 ->
+    push_var s st var val = (s', st') ->
+    lookup_s s' st' var = val.
+Proof.
+  intros.
+  assert (get_pred s' = pred (get_pred s)).
+  apply (add_stack_properly _ _ _ _ _ _ H H0 H1).
+  
+  destruct H.
+
+  (* we know that we cant have empty stack / table **)
+  destruct s; destruct st; try contradiction.
+
+  unfold push_var in H1. inversion H1; subst.
+
+  unfold push. unfold lookup_s.
+  unfold search_sm.
+
+  assert ((var !-> Some (get_pred s - Datatypes.length f); s0) var = Some (get_pred s - Datatypes.length f)).
+  apply update_eq.
+  rewrite H4; clear H4; simpl.
+  inversion H2; subst.
+
+  assert (get_pred s - Datatypes.length f -
+          S (get_pred s - S (Datatypes.length f)) = 0).
+  omega.
+  rewrite H4; clear.
+  reflexivity.
+Qed.
+
+(* Define a multi-step relationship **)
+
+Inductive cstack_seq : cstack -> stack sym_tbl -> cstack -> stack sym_tbl -> Prop :=
+| cstack_refl: forall s st,
+    cstack_seq s st s st
+| cstack_var: forall s s' st st' v val,
+    push_var s st v val = (s', st') ->
+    cstack_seq s st s' st'
+| cstack_frame: forall s s' st st',
+    push_new_frame s st = (s', st') ->
+    cstack_seq s st s' st'
+| cstack_trans: forall s s' s'' st st' st'',
+    cstack_seq s st s' st' ->
+    cstack_seq s' st' s'' st'' ->
+    cstack_seq s st s'' st''.
+
+Theorem backwards_validity_s: forall s s' st st',
+    s' <> [] /\ st' <> [] ->
+    get_pred s' <> 0 ->
+    cstack_seq s st s' st' ->
+    s <> [] /\ st <> [] /\ get_pred s <> 0.
+Proof.
+Admitted.
+
+Fixpoint shadowed (st: stack sym_tbl) (st': stack sym_tbl) v :=
+  match st' with
+  | [] => True (* Can't have new env bigger.  Impossible **)
+  | h::t => st <> st' /\ match h v with
+            | Some _ => True
+            | _ => shadowed st t v
+            end
+  end.
+
+(* Now, lemma showing that this works between frames **)
+Theorem lookup_works: forall (s s': cstack) (st st': stack sym_tbl) (v: string) (val: nat),
+    s' <> [] /\ st' <> [] ->
+    get_pred s' <> 0 ->
+    lookup_s s st v = val ->
+    cstack_seq s st s' st' ->
+    lookup_s s' st' v = val \/ shadowed st st' v. 
+Proof.
+Admitted.
+  
+  
+(* Finally, need some way to guarantee that removing frames doesn't break anything **)
+Theorem removal_works: forall (s s': cstack) (st st': stack sym_tbl) (v: string) (val: nat) f ft,
+    s <> [] /\ st <> [] ->
+    get_pred s <> 0 ->
+    lookup_s s st v = val ->
+    pop_frame s st = (f, s', ft, st') ->
+    lookup_s s st v = val \/ lookup_s [f] [ft] v = val.
+Proof.
+Admitted.
+
+(* No heap stuff yet **)
+
+  
+ 
+  
+  
+    
+    
+  
 
